moving around toString functions

thy/Common/Lib_toString.thy
@@ -16,6 +16,16 @@ definition string_of_int :: "int \<Rightarrow> string" where
 lemma "string_of_nat 123456 = ''123456''" by eval
 
 
+
+
+
+fun intersperse :: "'a \<Rightarrow> 'a list list \<Rightarrow> 'a list" where
+"intersperse _ [] = []" |
+"intersperse a [x] = x" |
+"intersperse a (x#xs) = x @ a # intersperse a xs"
+
+
+(*this is similar to space_implode or Data.List.intersperse (in Haskell)*)
 definition list_separated_toString :: "string \<Rightarrow> ('a \<Rightarrow> string) \<Rightarrow> 'a list \<Rightarrow> string" where
   "list_separated_toString sep toStr ls = concat (splice (map toStr ls) (replicate (length ls - 1) sep))"
 
@@ -24,13 +34,19 @@ fun list_separated_toString_helper :: "string \<Rightarrow> ('a \<Rightarrow> st
   "list_separated_toString_helper sep toStr [] = ''''" |
   "list_separated_toString_helper sep toStr [l] = toStr l" |
   "list_separated_toString_helper sep toStr (l#ls) = (toStr l)@sep@list_separated_toString_helper sep toStr ls"
-lemma "list_separated_toString = list_separated_toString_helper"
+lemma list_separated_toString_helper: "list_separated_toString = list_separated_toString_helper"
 proof -
   { fix sep and toStr::"('a \<Rightarrow> char list)" and ls
     have "list_separated_toString sep toStr ls = list_separated_toString_helper sep toStr ls"
       by(induction sep toStr ls rule: list_separated_toString_helper.induct) (simp_all add: list_separated_toString_def)
   } thus ?thesis by(simp add: fun_eq_iff)
 qed
+
+lemma list_separated_toString_intersperse:
+  "intersperse sep (map f xs) = list_separated_toString [sep] f xs"
+  apply(simp add: list_separated_toString_helper)
+  apply(induction "[sep]" f xs rule: list_separated_toString_helper.induct)
+    by simp+
 
 definition list_toString :: "('a \<Rightarrow> string) \<Rightarrow> 'a list \<Rightarrow> string" where
   "list_toString toStr ls = ''[''@ list_separated_toString '', '' toStr ls @'']''"
