thy/OpenFlow/OpenFlowSerialize.thy
@@ -1,53 +1,17 @@
 theory OpenFlowSerialize
-imports OpenFlowMatches OpenFlowAction Semantics_OpenFlow "../Primitive_Matchers/Common_Primitive_toString"
+imports OpenFlowMatches
+        OpenFlowAction
+        Semantics_OpenFlow
+        "../Common/Lib_toString"
+        "../Bitmagic/Lib_Word_toString"
+        "../Primitive_Matchers/Common_Primitive_toString"
 begin
 
 definition "serialization_test_entry \<equiv> OFEntry 7 {EtherDst 0x1, IPv4Dst (PrefixMatch 0xA000201 32), IngressPort ''s1-lan'', L4Dst 0x50 0, L4Src 0x400 0x3FF, IPv4Proto 6, EtherType 0x800} [ModifyField_l2dst 0xA641F185E862, Forward ''s1-wan'']"
 
-(*immitation of http://stackoverflow.com/questions/23864965/string-of-nat-in-isabelle*)
-definition "string_of_word_single lc w \<equiv> (if w < 10 then [char_of_nat (48 + unat w)] else if w < 36 then [char_of_nat ((if lc then 87 else 55) + unat w)] else undefined)"
-value "map (string_of_word_single False) (word_upto (-1) (36 :: 12 word))"
-function string_of_word :: "bool \<Rightarrow> ('a :: len) word \<Rightarrow> nat \<Rightarrow> ('a :: len) word \<Rightarrow> string" where (* lowercase?, base, minimum length - 1, to-be-serialized word *) 
-  "string_of_word lc base ml n = (if base < 2 \<or> len_of TYPE('a) < 2 then undefined else
-  	(if n < base \<and> ml = 0 then string_of_word_single lc n else string_of_word lc base (ml - 1) (n div base) @ string_of_word_single lc (n mod base)))"
-by clarsimp+
 
-value[code] "(0 :: nat) - 1"
-
-definition "hex_string_of_word l \<equiv> string_of_word True (16 :: ('a::len) word) l"
-definition "hex_string_of_word0 \<equiv> hex_string_of_word 0"
-(* be careful though, these functions only make sense with words > length 4. With 4 bits, base 16 is not representable. *)
-definition "dec_string_of_word0 \<equiv> string_of_word True 10 0"
-
-find_theorems "?a div (?b::('a :: len) word)"
-termination string_of_word
-	apply(relation "measure (\<lambda>(a,b,c,d). unat d + c)")
-	 apply(rule wf_measure)
-	apply(subst in_measure)
-	apply(clarsimp)
-	subgoal for base ml n
-    apply(case_tac "ml \<noteq> 0")
-     apply(simp add: less_eq_Suc_le unat_div)
-    apply(simp)
-    apply(subgoal_tac "(n div base) < n")
-     apply(blast intro: unat_mono)
-    apply(rule div_less_dividend_word)
-     subgoal by(metis Word_Lemmas.power_not_zero linorder_neqE_nat numeral_less_iff power_zero_numeral semiring_norm(76) word_neq_0_conv)
-    apply(clarsimp)
-    apply(thin_tac "n \<noteq> 0")
-    subgoal by (metis One_nat_def mult.right_neutral power_0 power_Suc unat_1 unat_power_lower Suc_1 inc_induct le_def less_eq_Suc_le lt1_neq0 not_degenerate_imp_2_neq_0 word_le_less_eq)
-  done
-done 
-
-value "hex_string_of_word0 (0xdeadbeef42 :: 42 word)"
-value "hex_string_of_word 1 (0x1 :: 5 word)"
 
 value "(map (op << (1::48 word) \<circ> op * 8) \<circ> rev) [0..<6]"
-
-fun intersperse where
-"intersperse _ [] = []" |
-"intersperse a [x] = x" |
-"intersperse a (x#xs) = x @ a # intersperse a xs"
 
 definition "serialize_mac (m::48 word) \<equiv> (intersperse (CHR '':'') \<circ> map (hex_string_of_word 1 \<circ> (\<lambda>h. (m >> h * 8) && 0xff)) \<circ> rev) [0..<6]"
 value "serialize_mac 0xdeadbeefcafe"
