thy/Bitmagic/Lib_Word_toString.thy
@@ -1,0 +1,45 @@
+theory Lib_Word_toString
+imports "../Common/Lib_toString"
+        "~~/src/HOL/Word/Word"
+        "./l4v/lib/Word_Lib/Word_Lemmas"
+begin
+
+(*immitation of http://stackoverflow.com/questions/23864965/string-of-nat-in-isabelle*)
+definition "string_of_word_single lc w \<equiv> (if w < 10 then [char_of_nat (48 + unat w)] else if w < 36 then [char_of_nat ((if lc then 87 else 55) + unat w)] else undefined)"
+value "map (string_of_word_single False) (word_upto (-1) (36 :: 12 word))"
+function string_of_word :: "bool \<Rightarrow> ('a :: len) word \<Rightarrow> nat \<Rightarrow> ('a :: len) word \<Rightarrow> string" where (* lowercase?, base, minimum length - 1, to-be-serialized word *) 
+  "string_of_word lc base ml n = (if base < 2 \<or> len_of TYPE('a) < 2 then undefined else
+  	(if n < base \<and> ml = 0 then string_of_word_single lc n else string_of_word lc base (ml - 1) (n div base) @ string_of_word_single lc (n mod base)))"
+by clarsimp+
+
+value[code] "(0 :: nat) - 1"
+
+definition "hex_string_of_word l \<equiv> string_of_word True (16 :: ('a::len) word) l"
+definition "hex_string_of_word0 \<equiv> hex_string_of_word 0"
+(* be careful though, these functions only make sense with words > length 4. With 4 bits, base 16 is not representable. *)
+definition "dec_string_of_word0 \<equiv> string_of_word True 10 0"
+
+find_theorems "?a div (?b::('a :: len) word)"
+termination string_of_word
+	apply(relation "measure (\<lambda>(a,b,c,d). unat d + c)")
+	 apply(rule wf_measure)
+	apply(subst in_measure)
+	apply(clarsimp)
+	subgoal for base ml n
+    apply(case_tac "ml \<noteq> 0")
+     apply(simp add: less_eq_Suc_le unat_div)
+    apply(simp)
+    apply(subgoal_tac "(n div base) < n")
+     apply(blast intro: unat_mono)
+    apply(rule div_less_dividend_word)
+     subgoal by(metis Word_Lemmas.power_not_zero linorder_neqE_nat numeral_less_iff power_zero_numeral semiring_norm(76) word_neq_0_conv)
+    apply(clarsimp)
+    apply(thin_tac "n \<noteq> 0")
+    subgoal by (metis One_nat_def mult.right_neutral power_0 power_Suc unat_1 unat_power_lower Suc_1 inc_induct le_def less_eq_Suc_le lt1_neq0 not_degenerate_imp_2_neq_0 word_le_less_eq)
+  done
+done 
+
+value "hex_string_of_word0 (0xdeadbeef42 :: 42 word)"
+value "hex_string_of_word 1 (0x1 :: 5 word)"
+
+end
